more work on find_path

verif/btrees/btrees.c
@@ -13,8 +13,8 @@ typedef struct node node;
 
 struct btree {
   struct node* root;
-  unsigned int num_records;
-  unsigned int depth;
+  int num_records;
+  int depth;
 };
 
 struct entry {
@@ -54,7 +54,7 @@ struct btree* new_btree() {
 
 void* ptr_at(node *n, int i) {
   if(i < 0) return (void*) n->ptr0;
-  else if (i >= 2*PARAM) return NULL;
+  else if (i >= (int) n->num_keys) return NULL;
   else return n->entries[i].ptr;
 };
 
@@ -67,26 +67,8 @@ void down_to_first(cursor *c) {
   };
 };
 
-void move_to_first(cursor *c) {
-  while(c->level > 0 && c->ancestors[c->level].index > 0)
-    c->level--;
-  c->ancestors[c->level].index = c->ancestors[c->level].node->is_leaf ? 0 : -1;
-  down_to_first(c);
-  return;
-};
-
-cursor* new_cursor(struct btree *t) {
-  cursor *c;
-  if(! (c = malloc(sizeof(cursor)))) exit(1);
-  c->btree = t;
-  c->level = 0;
-  c->ancestors[0].node = t->root;
-  move_to_first(c);
-  return c;
-};
-
 void move_to_next(cursor *c) {
-  while(c->level > 0 && c->ancestors[c->level].index >= c->ancestors[c->level].node->num_keys - 1)
+  while(c->level > 0 && c->ancestors[c->level].index >= (int) c->ancestors[c->level].node->num_keys - 1)
     c->level--;
 
   if(c->ancestors[c->level].index >= (int) c->ancestors[c->level].node->num_keys - 1)
@@ -101,10 +83,10 @@ void move_to_next(cursor *c) {
 int find_index(node *n, key k) {
   int i = 0;
   if(n->is_leaf) {
-    while(i < n->num_keys && n->entries[i].key < k) i++;
+    while(i < (int) n->num_keys && n->entries[i].key < k) i++;
     return i;
   } else {
-    while(i < n->num_keys && n->entries[i].key <= k) i++;
+    while(i < (int) n->num_keys && n->entries[i].key <= k) i++;
     return (i-1);
   };
 };
@@ -125,23 +107,23 @@ void move_to_key(cursor *c, key k) {
   return;
 };
 
+cursor* new_cursor(struct btree *t) {
+  cursor *c;
+  if(! (c = malloc(sizeof(cursor)))) exit(1);
+  c->btree = t;
+  c->level = 0;
+  c->ancestors[0].node = t->root;
+  move_to_key(c, 0);
+  return c;
+};
+
 void* get(cursor *c, key k) {
   move_to_key(c, k);
   return ptr_at(c->ancestors[c->level].node, c->ancestors[c->level].index);
 };
 
-void init(cursor *c) {
-  move_to_first(c);
-};
-
-void* next(cursor *c) {
-  void *rec = ptr_at(c->ancestors[c->level].node, c->ancestors[c->level].index);
-  move_to_next(c);
-  return rec;
-};
-
 void insert_entry(node *n, unsigned int i, key k, void* ptr) {
-  int c;
+  unsigned int c;
   for(c = n->num_keys; c > i; c--)
     n->entries[c] = n->entries[c-1]; // shift
     
@@ -179,7 +161,7 @@ void insert_aux(cursor *c, int level, key k, void* ptr) {
   node *n = c->ancestors[level].node;
 
   if(n->is_leaf) {
-    if(i < n->num_keys && n->entries[i].key == k) n->entries[i].ptr = ptr; // update
+    if(i < (int) n->num_keys && n->entries[i].key == k) n->entries[i].ptr = ptr; // update
     else if(n->num_keys < 2*PARAM) {
       insert_entry(n, i, k, ptr);
       c->btree->num_records++;
@@ -226,7 +208,7 @@ int main() {
   struct btree *t = new_btree();
   cursor *c = new_cursor(t);
 
-  for(int i = 0; i < 100; i++) insert(c, 2*i, NULL);
+  for(int i = 99; i >= 0; i--) insert(c, 2*i, NULL);
 
   insert(c, 11, NULL);
   insert(c, 33, NULL);
