verif/btrees/btrees_functional.v
@@ -1,6 +1,7 @@
 Require Import VST.floyd.functional_base.
-Require Import VST.floyd.proofauto.
+Require Import VST.veric.val_lemmas.
 Require Import VST.progs.conclib.
+Require Import VST.floyd.sublist.
 Require Import Program.Basics. (* for compose *)
 Require Import Program.Combinators. (* for compose notation "∘" *)
 
@@ -29,16 +30,77 @@ Qed.
 
 Unset Elimination Schemes.
 Inductive node: Type :=
-| leaf: forall (records: list (K * V)) (address: val), node
-| internal: forall (ptr0: node) (children: list (K * node)) (address: val), node.
+| leaf: forall (entries: list (K * V)) (address: val), node
+| internal: forall (ptr0: node) (entries: list (K * node)) (address: val), node.
 
-Inductive balanced: Z -> node -> Prop :=
-| balanced_leaf: forall {l p}, balanced 0 (leaf l p)
-| balanced_internal: forall {d ptr0 l p}, balanced d ptr0 -> Forall (balanced d ∘ snd) l ->
-                                     balanced (Z.succ d) (internal ptr0 l p). 
+Lemma node_ind (P: node -> Prop)
+      (hleaf: forall entries address, P (leaf entries address))
+      (hinternal: forall ptr0 entries address, P ptr0 -> Forall P (map snd entries) ->
+                                          P (internal ptr0 entries address)) : forall n, P n.
+Proof.
+  fix hrec 1.
+  intros [].
+  apply hleaf.
+  apply hinternal. apply hrec.
+  induction entries as [|[k n] entries]. constructor.
+  constructor. cbn. apply hrec. assumption.
+Qed.
+
+Inductive direct_subnode: relation node :=
+| subnode_ptr0: forall n ptr0 entries address,
+    direct_subnode n (internal ptr0 entries address)
+| subnode_entry: forall n ptr0 entries address m,
+    In m (map snd entries) ->
+    direct_subnode n (internal ptr0 entries address).
+
+Definition subnode: relation node := clos_refl_trans node direct_subnode.
 
 Instance Inhabitant_node: Inhabitant node :=
   leaf (combine (upto (Z.to_nat param)) (Zrepeat param nullV)) nullval.
+
+Inductive balanced: Z -> node -> Prop :=
+| balanced_leaf: forall {entries address}, balanced 0 (leaf entries address)
+| balanced_internal: forall {depth ptr0 entries address},
+    balanced depth ptr0 -> Forall (balanced depth ∘ snd) entries ->
+    balanced (Z.succ depth) (internal ptr0 entries address). 
+
+Lemma inv_balanced_leaf: forall depth entries address,
+    balanced depth (leaf entries address) ->
+    depth = 0.
+Proof. intros * h. inversion h. reflexivity. Qed.
+
+Lemma inv_balanced_internal: forall depth ptr0 entries address,
+    balanced depth (internal ptr0 entries address) ->
+    balanced (depth - 1) ptr0 /\ Forall (balanced (depth - 1) ∘ snd) entries.
+Proof. intros * h. inversion h.
+       replace (Z.succ depth0 - 1) with depth0 by omega.
+       auto.
+Qed.
+
+Lemma depth_nonneg: forall n depth, balanced depth n -> depth >= 0.
+Proof.
+  apply (node_ind (fun n => forall depth, balanced depth n -> depth >= 0)).
+  + intros * h. now inversion h.
+  + intros * hptr0 hentries depth hbal%inv_balanced_internal.
+    specialize (hptr0 _ (proj1 hbal)). omega.
+Qed.
+
+Inductive good_node: node -> Prop :=
+| good_leaf: forall entries address,
+    param <= Zlength entries <= 2*param ->
+    good_node (leaf entries address)
+| good_internal: forall ptr0 entries address,
+    param <= Zlength entries <= 2*param ->
+    good_node ptr0 ->
+    Forall (good_node ∘ snd) entries ->
+    good_node (internal ptr0 entries address).
+
+Fixpoint good_root (root: node): Prop :=
+  match root with
+  | leaf entries address => Zlength entries <= 2*param
+  | internal ptr0 entries address =>
+    1 <= Zlength entries <= 2*param /\ good_node ptr0 /\ Forall (good_node ∘ snd) entries
+  end.
 
 Definition is_leaf (n: node): Prop :=
   match n with
@@ -54,61 +116,253 @@ Definition is_leaf_dec (n: node): {is_leaf n} + {not (is_leaf n)} :=
 
 Definition keys (n: node): list K := 
   match n with
-  | leaf recs _ => map fst recs
-  | internal _ children _ => map fst children
+  | leaf entries _ | internal _ entries _ => map fst entries
   end.
 
 Definition node_address (n: node): val := 
-  match n with | leaf _ p => p | internal _ _ p => p end.
+  match n with | leaf _ address | internal _ _ address => address end.
 
 Arguments node_address n: simpl nomatch.
 
-Definition num_keys (n: node): Z :=
-  match n with leaf l _ => Zlength l | internal _ l _ => Zlength l end.
+Definition num_keys (n: node): Z := Zlength (keys n).
 
-(* Abstracting a node to an ordered list of (key,value) pairs *)
-Fixpoint abs_node (n: node): list (K * V) :=
+(* Abstracting a node to an ordered list of (key, value) pairs *)
+Fixpoint flatten (n: node): list (K * V) :=
   match n with
-  | leaf le _ => le
-  | internal ptr0 le _ => abs_node ptr0 ++ flat_map (abs_node ∘ snd) le
+  | leaf entries _ => entries
+  | internal ptr0 entries _ => flatten ptr0 ++ flat_map (flatten ∘ snd) entries
   end.
 
 Fixpoint num_records (n: node): Z :=
   match n with
-  | leaf le _ => Zlength le
-  | internal ptr0 le _ => num_records ptr0 + fold_right Z.add 0 (map (num_records ∘ snd) le)
+  | leaf entries _ => Zlength entries
+  | internal ptr0 entries _ => num_records ptr0 + fold_right Z.add 0 (map (num_records ∘ snd) entries)
   end.
 
-Lemma node_ind (P: node -> Prop)
-      (hleaf: forall l p, P (leaf l p))
-      (hinternal: forall ptr0 l p, P ptr0 -> Forall (P ∘ snd) l -> P (internal ptr0 l p)) : forall n, P n.
+Lemma num_records_flatten_length n : Zlength (flatten n) = num_records n.
 Proof.
-  fix hrec 1.
-  intros [].
-  apply hleaf.
-  apply hinternal. apply hrec.
-  induction children as [|[k n] children]. constructor.
-  constructor. cbn. apply hrec. assumption.
-Qed.
-
-Lemma numrec_abs_node_length n : Zlength (abs_node n) = num_records n.
-Proof.
-  apply (node_ind (fun n => Zlength (abs_node n) = num_records n)).
+  apply (node_ind (fun n => Zlength (flatten n) = num_records n)).
   + intros. reflexivity.
   + intros * hlength hforall.
     simpl. rewrite Zlength_app, hlength, flat_map_concat_map, Zlength_concat,
            map_map. do 2 f_equal.
     apply map_ext_in.
     intros [k n']. rewrite Forall_forall in hforall.
-    apply hforall.
+    intro hin. eapply in_map in hin.
+    apply hforall. eassumption.
 Qed.
 
-Inductive cursor: forall (root: node), Type :=
-| leaf_cursor: forall {l p} (k: K) (ptr: V) (i: Z)
-                 (hi: 0 <= i < Zlength l)
-                 (h: Znth i l = (k, ptr)), cursor (leaf l p) 
-| ptr0_cursor: forall {ptr0: node} {l p} (tl: cursor ptr0), cursor (internal ptr0 l p)
-| le_child_cursor: forall {ptr0 l p} (k: K) (child: node) (i: Z)
-                     (hi: 0 <= i < Zlength l)
-                     (h: Znth i l = (k, child))
-                     (tl: cursor child), cursor (internal ptr0 l p).
+Fixpoint find_path (key: K) (root: node) {struct root}: list (Z * node) :=
+match root with
+| leaf entries address =>
+  let index := (fix get_index entries index :=
+     match entries with
+     | [] => index
+     | (k, r) :: entries => if k >=? key then index else get_index entries (index + 1)
+  end) entries 0 in [(index, root)]
+| internal ptr0 (((first_k, first_n) :: _) as entries) address =>
+  if key <? first_k then (-1, root) :: find_path key ptr0 else
+    (fix get_cursor_entry entries index :=
+       match entries with
+       | [] => [] (* impossible case *)
+       | [(k, n)] => (index, root) :: find_path key n
+       | (k, n) :: (((k', n') :: _) as entries) =>
+         if ((k <=? key) && (key <? k'))%bool then (index, root) :: find_path key n
+         else get_cursor_entry entries (index + 1)
+       end) entries 0
+| internal ptr0 [] p => (-1, root) :: find_path key ptr0
+end.
+
+Lemma find_path_leaf: forall key entries address,
+    exists i, find_path key (leaf entries address) = [(i, leaf entries address)] /\
+         0 <= i <= Zlength entries /\
+         Forall (fun '(k, _) => k < key) (sublist 0 i entries) /\
+         (i < Zlength entries -> fst (Znth i entries) >= key).
+Proof.
+  intros.
+  pose (i entries z := (fix get_index (entries0 : list (Z * V)) (index : Z) {struct entries0} : Z :=
+         match entries0 with
+         | [] => index
+         | (k, _) :: entries1 => if k >=? key then index else get_index entries1 (index + 1)
+         end) entries z).
+  
+  assert (hadd: forall entries z, i entries z = i entries 0 + z).
+  { intro l; induction l as [|[k n] l]; simpl; intro z.
+    omega.
+    destruct Z.geb. omega.
+    rewrite (IHl (z + 1)), (IHl 1).
+    omega. }
+  
+  assert (hbounds: forall entries, 0 <= i entries 0 <= Zlength entries).
+  { intro l; induction l as [|[k' n'] l]; simpl.
+    - easy.
+    - rewrite Zlength_cons. destruct Z.geb. rep_omega.
+      rewrite hadd.
+      destruct (dec_Zgt (Zlength l) 0) as [hgt|hngt]; omega. }
+
+  assert (hforall: Forall (fun '(k, _) => k < key) (sublist 0 (i entries 0) entries)).
+  { induction entries as [|[k n] entries].
+    rewrite sublist_nil_gen. constructor.
+    unfold i; omega.
+    case_eq (k >=? key); intro hbool. rewrite sublist_nil_gen. constructor. unfold i. rewrite hbool. omega.
+    rewrite sublist_0_cons'. constructor. rewrite <- Z.leb_gt, <- Z.geb_leb. assumption.
+    replace (sublist 0 (i ((k, n) :: entries) 0 - 1) entries) with
+        (sublist 0 (i ((k, n) :: entries) 0 - 1) (sublist 0 (i entries 0) entries)).
+    apply Forall_sublist, IHentries.
+    rewrite sublist_sublist00. reflexivity. simpl. rewrite hbool.
+    rewrite hadd. specialize (hbounds entries). omega. omega.
+    simpl. rewrite hbool. rewrite hadd. specialize (hbounds entries). omega. }
+
+  exists (i entries 0); split3; auto; split; auto.
+  { clear hforall; induction entries as [|[k n] entries].
+    easy.
+    simpl. case_eq (k >=? key). intros hb%Z.geb_le _. simpl. omega.
+    intros hb h. rewrite hadd, Znth_pos_cons.
+    replace (_ + 1 - 1) with (i entries 0) by omega.
+    apply IHentries. rewrite Zlength_cons, hadd in h. omega.
+    specialize (hbounds entries); omega. }
+Qed.
+
+Lemma find_path_internal: forall key ptr0 entries address,
+    exists i, find_path key (internal ptr0 entries address) =
+         (i, internal ptr0 entries address) :: find_path key (@Znth _ ptr0 i (map snd entries)) /\
+         -1 <= i < Zlength entries /\
+         Forall (fun '(k, _) => k <= key) (sublist 0 (i + 1) entries) /\
+         (i + 1 < Zlength entries -> key < Znth (i + 1) (map fst entries)).
+Proof.
+  intros.
+  destruct entries as [|[first_k first_n] entries]; simpl.
+  + exists (-1). split3.
+    - reflexivity.
+    - rewrite Zlength_nil; omega.
+    - now rewrite sublist_of_nil, Zlength_nil, Znth_nil.
+  + case_eq (key <? first_k); simpl; intro hb.
+    - exists (-1). rewrite Zlength_cons, Znth_underflow, sublist_nil, Znth_0_cons by omega.
+      split3; try easy; try rep_omega.
+      split. constructor. intros _. now rewrite Z.ltb_lt in hb.
+    - generalize (internal ptr0 ((first_k, first_n) :: entries) address) as root.
+      revert hb.
+      generalize first_k as k, first_n as n. clear first_k first_n. intros.
+
+      pose (i l z := (fix get_index (l : list (K * node)) index :=
+                     match l with
+                     | [] => index
+                     | [(k, n)] => index
+                     | (k, _) :: ((k', _) :: _) as tl =>
+                       if ((k <=? key) && (key <? k'))%bool
+                       then index
+                       else get_index tl (index + 1)
+                     end) l z).
+      
+      assert (hadd: forall l z, i l z = i l 0 + z).
+      { induction l as [|[k' n'] l]; intros; simpl.
+        omega.
+        destruct l as [|[k'' n''] l]. omega.
+        destruct andb. omega. rewrite (IHl (z + 1)), (IHl 1). omega. }
+      
+      assert (hbounds: forall l k n z, z <= i ((k, n) :: l) z < z + 1 + Zlength l).
+      { induction l as [|[k' n'] l]; intros. simpl.
+        rewrite Zlength_nil; simpl; omega.
+        specialize (IHl k' n' (z + 1)). rewrite Zlength_cons; simpl in IHl |- *.
+        destruct andb; rep_omega. }
+      
+      exists (i ((k, n) :: entries) 0).
+      split3.
+      ++ generalize k as k0, n as n0.
+         change 1 with (0 + 1) at 2.
+         generalize 0 at -5 as z.
+         induction entries as [|[k0 n0] entries]; intros.
+         reflexivity.
+         simpl; case_eq ((k1 <=? key) && (key <? k0))%bool; intro hb'.
+         reflexivity.
+         simpl in hadd.
+         rewrite IHentries.
+         rewrite (Znth_pos_cons _ (n0 :: _)).
+         simpl. 
+         specialize (hadd ((k0, n0) :: entries) 1). simpl in hadd.
+         rewrite hadd. rewrite <- Z.add_sub_assoc, Z.sub_diag, Z.add_0_r. reflexivity. 
+         destruct entries as [|[k2 n2] entries]. omega.
+         destruct ((k0 <=? key) && (key <? k2))%bool. omega. specialize (hbounds entries k2 n2 2). omega.
+      ++ pose proof (hbounds entries k n 0) as h.
+         rewrite Zlength_cons; omega.
+      ++ split.
+      -- revert hb. generalize k as k0, n as n0. 
+         induction entries as [|[k' n'] entries]; intros.
+         cbn. constructor. rewrite <- Z.ltb_ge. assumption. constructor.
+         specialize (IHentries k' n').
+         rewrite <- hadd in IHentries.
+         pose proof (hbounds entries k n 1). pose proof (hbounds entries k' n' 1).
+         simpl in *. rewrite sublist_0_cons in IHentries by rep_omega.
+         case_eq ((k0 <=? key) && (key <? k'))%bool; intro hb'.
+         cbn. constructor. rewrite <- Z.ltb_ge. assumption. constructor.
+         assert (hk': k' <= key).
+         {  rewrite andb_false_iff in hb'.
+            rewrite Z.ltb_ge in hb', hb. rewrite Z.leb_gt in hb'. destruct hb'. omega. assumption. }
+         rewrite sublist_0_cons by rep_omega.
+         constructor. rewrite <- Z.ltb_ge. assumption.
+         rewrite <- Z.add_sub_assoc, Z.sub_diag, Z.add_0_r, sublist_0_cons by rep_omega.
+         constructor. assumption.
+         rewrite <- Z.ltb_ge in hk'. specialize (IHentries hk').
+         inversion IHentries. assumption.
+      -- revert hb. generalize k. induction entries as [|[k' n'] entries]. 
+         cbn; intros; omega.
+         simpl; intros k_ hk_.
+         specialize (IHentries k'). specialize (hbounds entries k' n' 1).
+         case_eq ((k_ <=? key) && (key <? k'))%bool; intros hb h.
+         * simpl. rewrite Znth_pos_cons, Znth_0_cons by omega.
+           rewrite andb_true_iff in hb. destruct hb. rewrite <- Z.ltb_lt. assumption.
+         * rewrite <- hadd in IHentries. simpl in IHentries.
+           rewrite Znth_pos_cons. rewrite <- Z.add_sub_assoc, Z.sub_diag, Z.add_0_r.
+           apply IHentries. rewrite andb_false_iff in hb. destruct hb.
+           rewrite Z.ltb_ge in hk_. rewrite Z.leb_gt in H. omega.
+           assumption. rewrite Zlength_cons, Zlength_cons in h.
+           rewrite Zlength_cons. rep_omega.
+           simpl in hbounds. rep_omega.
+Qed.
+
+Require Import Sorting.Sorted.
+
+Lemma find_path_is_path: forall key root depth,
+    balanced depth root ->
+    Sorted (flip direct_subnode) (map snd (find_path key root)).
+Proof.
+  intro key.
+  apply (node_ind (fun root => forall depth, balanced depth root -> Sorted (flip direct_subnode) (map snd (find_path key root)))).
+  + repeat constructor.
+  + intros * hptr0 hentries depth hbalanced.
+    pose proof (find_path_internal key ptr0 entries address) as hfp.
+    destruct hfp as [i (heq & hbounds & hbefore & hafter)].
+    rewrite heq.
+    Admitted.
+    
+
+Lemma find_path_subnode: forall key root n,
+    In n (map snd (find_path key root)) -> subnode n root.
+Proof.
+  intro key. apply (node_ind (fun root => forall n, In n (map snd (find_path key root)) -> subnode n root)).
+  + intros * hin. replace n with (leaf entries address). constructor.
+    symmetry. replace (map snd (find_path key (leaf entries address))) with [leaf entries address] in hin.
+    now inversion hin. clear hin.
+    induction entries as [|[k r] entries].
+    reflexivity.
+    cbn.
+    intros hin. destruct hin. subst. constructor. contradiction.
+    cbn in hin.
+    destruct (k >=? key). inversion hin. subst. reflexivity. contradiction.
+    
+  intros * hin.
+  
+
+Section Tests.
+
+  Definition aux (l: list K): list (K * V) := map (fun k => (k, nullV)) l.
+  
+  Definition test_node: node :=
+    internal (leaf (aux [1; 2; 3]) nullval)
+             [(4, leaf (aux [4; 5; 6]) nullval);
+              (7, leaf (aux [7; 8; 9]) nullval);
+              (10, leaf (aux [10; 11; 12]) nullval)] nullval.
+
+  Timeout 20 Compute (find_path 11 test_node).
+
+End Tests.
