verif/btrees/btrees_spec.v
@@ -9,6 +9,8 @@ Definition Vprog : varspecs. mk_varspecs prog. Defined.
 Require Import btrees_functional.
 Require Import btrees_sep.
 
+Require Import Program.Basics. Require Import Program.Combinators.
+
 Definition new_btree_spec : ident * funspec :=
   DECLARE _new_btree
   WITH gv: globals
@@ -26,7 +28,8 @@ Definition ptr_at_spec : ident * funspec :=
   DECLARE _ptr_at
   WITH gv: globals, n: node, i: Z
   PRE [ _n OF tptr tnode, _i OF tint ]
-         PROP (Int.min_signed <= i <= Int.max_signed; i < num_keys n <= 2*param)
+         PROP (Int.min_signed <= i <= Int.max_signed;
+              num_keys n <= 2*param)
          LOCAL (gvars gv; temp _n (node_address n); temp _i (vint i))
          SEP (mem_mgr gv; node_rep n)
   POST [ tptr tvoid ]
@@ -39,12 +42,62 @@ Definition ptr_at_spec : ident * funspec :=
          LOCAL (temp ret_temp res)
          SEP (mem_mgr gv; node_rep n).
 
+Definition move_to_key_spec : ident * funspec :=
+  DECLARE _move_to_key
+  WITH gv: globals, pc: val, root: node, old_k: K, k: K, depth: Z
+  PRE [ _c OF tptr tcursor, _k OF tuint ]
+         PROP (depth < 20; balanced depth root)
+         LOCAL (gvars gv; temp _c pc; temp _k (vint k))
+         SEP (mem_mgr gv; cursor_rep old_k root pc; node_rep root)
+  POST [ tvoid ]
+         PROP ()
+         LOCAL ()
+         SEP (mem_mgr gv; cursor_rep k root pc; node_rep root).
+
+(*
+Definition down_to_first_spec : ident * funspec :=
+  DECLARE _down_to_first
+  WITH gv: globals, pc: val, c_sigT: { root: node & cursor root }
+  PRE [ _c OF tptr tcursor ]
+         PROP (balanced depth (projT1 root_sigT))
+         LOCAL (gvars gv; temp _c pc)
+         SEP (mem_mgr gv; cursor_rep level (projT2 root_sigT) pc; node_rep (projT1 root_sigT))
+  POST [ tvoid ]
+         PROP ()
+         LOCAL ()
+         SEP (mem_mgr gv; cursor_rep depth (down_to_first (projT2 root_sigT)); node_rep (projT1 rc)).
+*)
 Definition Gprog : funspecs :=
-        ltac:(with_library prog [ new_btree_spec ]).
+        ltac:(with_library prog [ new_btree_spec; ptr_at_spec; move_to_key_spec ]).
 
 Set Default Timeout 20.
 Arguments proj_reptype _ _ _ v: simpl never.
-Arguments force_lengthn A n xs default: simpl never.
+
+Lemma body_move_to_key: semax_body Vprog Gprog f_move_to_key move_to_key_spec.
+Proof.
+  start_function.
+  forward_loop
+    (EX level: Z,
+     PROP (0 <= level <= Zlength (find_path old_k root) - 1)
+     LOCAL (gvars gv; temp _c pc)
+     SEP (mem_mgr gv; partial_cursor_rep old_k root level pc; node_rep root))
+    break: (EX level: Z,
+            PROP (level <= 0 \/ sublist 0 (level + 1) (find_path old_k root) = sublist 0 (level + 1) (find_path k root))
+            LOCAL ()
+            SEP (partial_cursor_rep old_k root level pc)).
+  + Exists (Zlength (find_path old_k root) - 1). entailer!. rewrite (find_path_Zlength _ _ _ H0).
+    apply depth_nonneg in H0. omega. apply derives_refl.
+  + unfold partial_cursor_rep. Intros level ptree.
+    forward.
+    forward_if (PROP ()
+                LOCAL (gvars gv; temp _c pc)
+                SEP (mem_mgr gv;
+                data_at Ews tcursor
+                        (ptree,
+                         (vint level,
+                          complete max_depth (map (fun '(i0, n) => (vint i0, node_address n)) (find_path old_k root)))) pc; node_rep root)).
+  - forward. forward. rewrite (find_path_Zlength _ _ _ H0) in H1. entailer!.
+    entailer!.
 
 Lemma body_ptr_at: semax_body Vprog Gprog f_ptr_at ptr_at_spec.
 Proof.
@@ -55,28 +108,32 @@ Proof.
     { apply prop_right. rewrite Znth_underflow. reflexivity. rep_omega. }
     { entailer!. rewrite Zaux.Zlt_bool_true by assumption. reflexivity.
     unfold node_rep; fold node_rep. entailer!. }
-  + forward_if.
-    - forward.
-    - destruct n; unfold node_address, node_rep; fold node_rep;
-      Intros.
-      { assert (h: snd (Znth i (complete 17 (map (fun '(k, ptr) => (vint k, proj1_sig ptr)) records))) = proj1_sig (snd (Znth i records))).
-        { simpl in H0. destruct H0.
-          rewrite Znth_complete, Znth_map by
-          (try rewrite Zlength_map; fold K V; rep_omega).  now destruct Znth. }
-        forward. entailer!. setoid_rewrite h. now destruct (snd (Znth i records)).
-        forward. }
-      { simpl in H0. destruct H0.
-        assert (h: snd (Znth i (complete 17 (map (fun '(k, ptr) => (vint k, node_address ptr)) children))) = node_address (snd (Znth i children))).
-        { rewrite Znth_complete, Znth_map by
-              (try rewrite Zlength_map; fold K V; rep_omega).  now destruct Znth. }
-        forward. entailer. setoid_rewrite h.
-        rewrite iter_sepcon_Znth with (i0 := i) by rep_omega. cbn. entailer.
-        forward.
-        setoid_rewrite h. rewrite Zaux.Zlt_bool_false by omega. cbn.
-        entailer!.
-      }
-Qed.
+  + assert (Int.min_signed <= num_keys n <= Int.max_signed).
+    { split. destruct n; simpl num_keys; rep_omega. rep_omega. }
 
+    destruct n; simpl node_rep; simpl node_address; simpl in H0; Intros.
+    - forward. forward_if.
+      ++ forward. apply prop_right.
+         rewrite Znth_overflow by assumption. reflexivity.
+      ++ assert (h: snd (Znth i (complete 17 (map (fun '(k, ptr) => (vint k, proj1_sig ptr)) records))) = proj1_sig (snd (Znth i records))).
+           { rewrite Znth_complete, Znth_map by
+                 (try rewrite Zlength_map; fold K V; rep_omega).  now destruct Znth. }
+         forward.
+         entailer. apply prop_right. setoid_rewrite h. now destruct (snd (Znth i records)).
+         forward.
+    - forward. forward_if.
+      ++ forward. simpl node_rep. entailer!.
+         rewrite Znth_overflow by assumption. rewrite Zaux.Zlt_bool_false by rep_omega.
+         reflexivity.
+      ++ assert (h: snd (Znth i (complete 17 (map (fun '(k, child) => (vint k, node_address child)) children))) = node_address (snd (Znth i children))).
+           { rewrite Znth_complete, Znth_map by
+                 (try rewrite Zlength_map; fold K V; rep_omega). now destruct Znth. }
+         forward.
+         entailer. setoid_rewrite h.
+         rewrite iter_sepcon_Znth with (i0 := i) by rep_omega.
+         unfold compose. destruct (snd (Znth i children)); simpl; entailer.
+         forward. setoid_rewrite h. rewrite Zaux.Zlt_bool_false by omega. simpl. entailer!.
+Qed.
 
 Lemma body_new_btree: semax_body Vprog Gprog f_new_btree new_btree_spec.
 Proof.
@@ -108,7 +165,8 @@ Proof.
   - rewrite if_false by assumption.
     forward. entailer!.
   - do 9 forward.
-    unfold btree_rep, node_rep, node_address. 
+    unfold btree_rep, node_rep, node_address.
     Exists p p_root.
     entailer!.
 Qed.
+n
